clean up. Consistency. Hocap spec somewhat written in. Need to change style so viewshift is in precondition.

theories/twoLockMSQ_hocap_spec.v
@@ -43,14 +43,12 @@ Definition TokBefore (g : Qgnames) := token g.(γ_Before).
 Definition TokAfter (g : Qgnames) := token g.(γ_After).
 Definition TokUpdated (g : Qgnames) := ((TokBefore g) ∗ (TokAfter g))%I.
 
-(* TODO: write in correct invariant *)
-Definition queue_invariant (Ψ : val -> iProp Σ) (l_head l_tail : loc) (Q_γ : Qgnames) : iProp Σ :=
-	∃ xs_v, (* Abstract state *)
+Definition queue_invariant (l_head l_tail : loc) (Q_γ : Qgnames) : iProp Σ :=
+	∃ xs_v, own Q_γ.(γ_Abst) (●F (to_agree xs_v)) ∗ (* Abstract state *)
 	∃ xs xs_queue xs_old (x_head x_tail: (loc * val * loc)), (* Concrete state *)
 	⌜xs = xs_queue ++ [x_head] ++ xs_old⌝ ∗
 	isLL xs ∗
 	⌜proj_val xs_queue = wrap_some xs_v⌝ ∗
-	All xs_v Ψ ∗
 	(
 		(* Static *)
 		(
@@ -85,13 +83,12 @@ Definition queue_invariant (Ψ : val -> iProp Σ) (l_head l_tail : loc) (Q_γ : 
 		)
 	).
 
-Definition queue_invariant_simple (Ψ : val -> iProp Σ) (l_head l_tail : loc) (Q_γ : Qgnames) : iProp Σ :=
-	∃ xs_v, (* Abstract state *)
+Definition queue_invariant_simple (l_head l_tail : loc) (Q_γ : Qgnames) : iProp Σ :=
+	∃ xs_v, own Q_γ.(γ_Abst) (●F (to_agree xs_v)) ∗ (* Abstract state *)
 	∃ xs xs_queue xs_old (x_head x_tail: (loc * val * loc)), (* Concrete state *)
 	⌜xs = xs_queue ++ [x_head] ++ xs_old⌝ ∗
 	isLL xs ∗
 	⌜proj_val xs_queue = wrap_some xs_v⌝ ∗
-	All xs_v Ψ ∗
 	(
 		(
 			(l_head ↦ #(n_in x_head) ∗ ToknD Q_γ) ∨ 
@@ -109,14 +106,14 @@ Definition queue_invariant_simple (Ψ : val -> iProp Σ) (l_head l_tail : loc) (
 		)
 	).
 
-Lemma queue_invariant_equiv_simple : forall Ψ l_head l_tail Q_γ,
-	(queue_invariant Ψ l_head l_tail Q_γ) ∗-∗
-	(queue_invariant_simple Ψ l_head l_tail Q_γ).
+Lemma queue_invariant_equiv_simple : forall l_head l_tail Q_γ,
+	(queue_invariant l_head l_tail Q_γ) ∗-∗
+	(queue_invariant_simple l_head l_tail Q_γ).
 Proof.
-	iIntros (Ψ l_head l_tail Q_γ).
+	iIntros (l_head l_tail Q_γ).
 	iSplit.
-	- iIntros "(%xs_v & %xs & %xs_queue & %xs_old & %x_head & %x_tail & Hxs_split & HisLL_xs & %Hconc_abst_eq & HAll & [H_Static | [H_Enqueue | [H_Dequeue | H_Both]]])"; 
-	iExists xs_v, xs, xs_queue, xs_old, x_head, x_tail; iFrame.
+	- iIntros "(%xs_v & HAbst_auth & %xs & %xs_queue & %xs_old & %x_head & %x_tail & Hxs_split & HisLL_xs & %Hconc_abst_eq & [H_Static | [H_Enqueue | [H_Dequeue | H_Both]]])"; 
+	iExists xs_v; iFrame; iExists xs, xs_queue, xs_old, x_head, x_tail; iFrame.
 	  + iDestruct "H_Static" as "(Hl_head & Hl_tail & HisLast & HTokne & HToknD & HTokUpdated)".
 	  	iSplit; first done.
 		iSplitL "Hl_head HToknD"; first (iLeft; iFrame).
@@ -139,44 +136,97 @@ Proof.
 		* iSplit; first done.
 		  iSplitL "Hl_head HTokD"; first (iRight; iFrame). 
 		  iRight. iFrame. iRight. iFrame.
-	- iIntros "(%xs_v & %xs & %xs_queue & %xs_old & %x_head & %x_tail & Hxs_split & HisLL_xs & %Hconc_abst_eq & HAll & [[Hl_head HToknD] | [Hl_head HTokD]] & [(Hl_tail & HisLast & HToknE & HTokUpdated) | (Hl_tail & HTokE & [[HisLast HTokBefore] | [HisSndLast HTokAfter]])])";
-	iExists xs_v, xs, xs_queue, xs_old, x_head, x_tail; eauto 10 with iFrame.
+	- iIntros "(%xs_v & HAbst_auth & %xs & %xs_queue & %xs_old & %x_head & %x_tail & Hxs_split & HisLL_xs & %Hconc_abst_eq & [[Hl_head HToknD] | [Hl_head HTokD]] & [(Hl_tail & HisLast & HToknE & HTokUpdated) | (Hl_tail & HTokE & [[HisLast HTokBefore] | [HisSndLast HTokAfter]])])";
+	iExists xs_v; iFrame; iExists xs, xs_queue, xs_old, x_head, x_tail; eauto 10 with iFrame.
 Qed.
 
-Definition is_queue (Ψ : val -> iProp Σ) (v_q : val) (Q_γ: Qgnames) : iProp Σ :=
+Definition is_queue (v_q : val) (Q_γ: Qgnames) : iProp Σ :=
 	∃ l_queue l_head l_tail : loc, ∃ H_lock T_lock : val,
 	⌜v_q = #l_queue⌝ ∗
 	l_queue ↦□ ((#l_head, #l_tail), (H_lock, T_lock)) ∗
-	inv N (queue_invariant Ψ l_head l_tail Q_γ) ∗
+	inv N (queue_invariant l_head l_tail Q_γ) ∗
 	is_lock Q_γ.(γ_Hlock) H_lock (TokD Q_γ) ∗
 	is_lock Q_γ.(γ_Tlock) T_lock (TokE Q_γ).
 
 (* is_queue is persistent *)
-Global Instance is_queue_persistent Ψ v_q Q_γ : Persistent (is_queue Ψ v_q Q_γ).
+Global Instance is_queue_persistent v_q Q_γ : Persistent (is_queue v_q Q_γ).
 Proof. apply _. Qed.
 
-(* Todo Write in spec *)
-
-Lemma initialize_spec (Ψ : val -> iProp Σ):
+Lemma initialize_spec:
 	{{{ True }}}
 		initialize #()
-	{{{ v_q Q_γ, RET v_q; is_queue Ψ v_q Q_γ }}}.
+	{{{ v_q Q_γ, RET v_q; is_queue v_q Q_γ ∗
+						  own Q_γ.(γ_Abst) (◯F (to_agree [])) }}}.
 Proof.
-	iIntros (Φ) "_ HΦ". Admitted.
+	iIntros (Φ) "_ HΦ".
+	wp_lam.
+	wp_pures.
+	wp_alloc l_1_out as "Hl_1_out".
+	wp_alloc l_1_in as "Hl_1_in".
+	wp_pures.
+	iMod (pointsto_persist with "Hl_1_in") as "#Hl_1_in".
+	wp_pures.
+	iMod token_alloc as (γ_D) "Hγ_D".
+	wp_apply (newlock_spec with "Hγ_D").
+	iIntros (hlock γ_Hlock) "Hγ_Hlock".
+	wp_let.
+	iMod token_alloc as (γ_E) "Hγ_E".
+	wp_apply (newlock_spec with "Hγ_E").
+	iIntros (tlock γ_Tlock) "Hγ_Tlock".
+	wp_let.
+	wp_alloc l_tail as "Hl_tail".
+	wp_alloc l_head as "Hl_head".
+	iMod token_alloc as (γ_nE) "Hγ_nE".
+	iMod token_alloc as (γ_nD) "Hγ_nD".
+	iMod token_alloc as (γ_Before) "Hγ_Before".
+	iMod token_alloc as (γ_After) "Hγ_After".
+	iMod (own_alloc (●F (to_agree []) ⋅ ◯F (to_agree []))) as (γ_Abst) "[Hγ_Abst_auth Hγ_Abst_frac]"; first by apply frac_auth_valid.
+	set (Queue_gnames := {| γ_Abst := γ_Abst;
+							γ_Hlock := γ_Hlock;
+							γ_Tlock := γ_Tlock;
+							γ_E := γ_E;
+							γ_nE := γ_nE;
+							γ_D := γ_D;
+							γ_nD := γ_nD;
+							γ_Before := γ_Before;
+							γ_After := γ_After
+					|}).
+	iMod (inv_alloc N _ (queue_invariant l_head l_tail Queue_gnames) with "[Hγ_Abst_auth Hl_head Hl_tail Hl_1_in Hl_1_out Hγ_nE Hγ_nD Hγ_Before Hγ_After]") as "#HqueueInv".
+	{
+		iNext. iExists []. iFrame. iExists [(l_1_in, NONEV, l_1_out)], [], [], (l_1_in, NONEV, l_1_out), (l_1_in, NONEV, l_1_out). cbn. iSplit; first done. iSplitL "Hl_1_in Hl_1_out"; first auto. iSplit; first done.
+		iLeft. iFrame. iPureIntro. by exists [].
+	}
+	wp_alloc l_queue as "Hl_queue".
+	iMod (pointsto_persist with "Hl_queue") as "#Hl_queue".
+	iApply ("HΦ" $! #l_queue Queue_gnames).
+	iModIntro.
+	iFrame.
+	iExists l_queue, l_head, l_tail, hlock, tlock.
+	by repeat iSplit.
+Qed.
 
-Lemma enqueue_spec v_q Ψ (v : val) (qg : Qgnames) :
-	{{{ is_queue Ψ v_q qg ∗ Ψ v }}}
+Lemma enqueue_spec v_q (v : val) (Q_γ : Qgnames) (P Q : iProp Σ) :
+	□(∀xs_v, (own Q_γ.(γ_Abst) (●F (to_agree xs_v)) ∗ P
+				={⊤ ∖ ↑N}=∗ own Q_γ.(γ_Abst) (●F (to_agree (v :: xs_v))) ∗ Q))
+	-∗
+	{{{ is_queue v_q Q_γ ∗ P}}}
 		enqueue v_q v
-	{{{ w, RET w; True }}}.
+	{{{ w, RET w; Q }}}.
 Proof.
 	Admitted.
 
-Lemma dequeue_spec P Q v_q Ψ (qg : Qgnames) :
-	{{{ (P ={⊤ ∖ ↑N}=∗ Q) ∗ own qg.(γ_Abst) (●F (to_agree [])) ∗ is_queue Ψ v_q qg }}}
+Lemma dequeue_spec v_q (Q_γ : Qgnames) (P : iProp Σ) (Q : val -> iProp Σ):
+	□(∀xs_v, (own Q_γ.(γ_Abst) (●F (to_agree xs_v)) ∗ P
+				={⊤ ∖ ↑N}=∗
+		      	(( ⌜xs_v = []⌝ ∗ own Q_γ.(γ_Abst) (●F (to_agree (xs_v))) ∗ Q NONEV) ∨
+				(∃x_v xs_v', ⌜xs_v = xs_v' ++ [x_v]⌝ ∗ own Q_γ.(γ_Abst) (●F (to_agree (xs_v'))) ∗ Q (SOMEV x_v)))
+			)
+	 )
+	-∗
+	{{{ is_queue v_q Q_γ ∗ P}}}
 		dequeue v_q
-	{{{ v, RET v; ⌜v = NONEV⌝ ∨ (∃ x_v, ⌜v = SOMEV x_v⌝ ∗ Ψ x_v) }}}.
+	{{{ v, RET v; Q v }}}.
 Proof.
-	iIntros (Φ) "H HΦ".
 	Admitted.
 
 End proofs.
